add: Sequent

Logic/Vorspiel/Collection.lean
@@ -1,48 +1,100 @@
 
 import Logic.Vorspiel.Vorspiel
 
-class Cons (β : outParam Type*) (α : Type*) where
-  cons : β → α → α
-export Cons (cons)
-
-instance (α : Type*) : Cons α (Set α) := ⟨insert⟩
-
-instance (α : Type*) : Cons α (List α) := ⟨List.cons⟩
-
-instance (α : Type*) : Cons α (Multiset α) := ⟨Multiset.cons⟩
-
-instance (α : Type*) [DecidableEq α] : Cons α (Finset α) := ⟨insert⟩
-
-class Collection (β : outParam Type*) (α : Type*) extends Membership β α, HasSubset α, EmptyCollection α, Cons β α where
+class Collection (β : outParam Type*) (α : Type*) extends Membership β α, HasSubset α, EmptyCollection α, Singleton β α where
   subset_iff {a b : α} : a ⊆ b ↔ ∀ x ∈ a, x ∈ b
-  not_mem_empty (x : β) : ¬x ∈ (∅ : α)
-  mem_cons_iff {x z : β} {a : α} : x ∈ cons z a ↔ x = z ∨ x ∈ a
+  not_mem_empty (x : β) : x ∉ (∅ : α)
+  mem_singleton {x z : β} : x ∈ ({z} : α) ↔ x = z
 
-attribute [simp] Collection.not_mem_empty Collection.mem_cons_iff
+attribute [simp] Collection.not_mem_empty
 
 instance Set.collection : Collection α (Set α) where
   subset_iff := iff_of_eq Set.subset_def
   not_mem_empty := by simp
-  mem_cons_iff := by simp [Cons.cons]
+  mem_singleton := by simp
 
 instance List.collection : Collection α (List α) where
   subset_iff := List.subset_def
   not_mem_empty := by simp
-  mem_cons_iff := by simp [Cons.cons]
+  mem_singleton := by simp [List.singleton_eq]
 
 instance Multiset.collection : Collection α (Multiset α) where
   subset_iff := Multiset.subset_iff
   not_mem_empty := by simp
-  mem_cons_iff := by simp [Cons.cons]
+  mem_singleton := by simp
 
 instance Finset.collection [DecidableEq α] : Collection α (Finset α) where
   subset_iff := Finset.subset_iff
   not_mem_empty := by simp
-  mem_cons_iff := by simp [Cons.cons]
+  mem_singleton := by simp
+
+namespace Option
+
+variable {α : Type*}
+
+inductive Subset : Option α → Option α → Prop where
+  | none_none : Subset none none
+  | none_some (a : α) : Subset none (some a)
+  | some_some (a : α) : Subset (some a) (some a)
+
+instance : HasSubset (Option α) := ⟨Subset⟩
+
+@[simp] lemma none_subset (o : Option α) : none ⊆ o := by
+  cases o
+  · exact Subset.none_none
+  · exact Subset.none_some _
+
+@[simp, refl] lemma Subset.refl (o : Option α) : o ⊆ o := by
+  cases o
+  · exact Subset.none_none
+  · exact Subset.some_some _
+
+@[simp] lemma some_subset_some_iff {a b : α} : some a ⊆ some b ↔ a = b := by
+  constructor
+  · rintro ⟨⟩; rfl
+  · rintro rfl; rfl
+
+@[trans] lemma Subset.trans {o₁ o₂ o₃ : Option α} : o₁ ⊆ o₂ → o₂ ⊆ o₃ → o₁ ⊆ o₃ := by
+  rintro ⟨⟩ ⟨⟩ <;> simp
+
+lemma subset_iff {o₁ o₂ : Option α} : o₁ ⊆ o₂ ↔ ∀ x ∈ o₁, x ∈ o₂ := by
+  cases o₁ <;> cases o₂ <;> simp [eq_comm]
+  · rintro ⟨⟩
+
+instance : EmptyCollection (Option α) := ⟨none⟩
+
+lemma empty_def : (∅ : Option α) = none := rfl
+
+instance : Singleton α (Option α) := ⟨some⟩
+
+lemma singleton_def (a : α) : ({a} : Option α) = some a := rfl
+
+end Option
+
+instance Option.collection : Collection α (Option α) where
+  subset_iff := by simp [Option.subset_iff]
+  not_mem_empty := by simp
+  mem_singleton := by simp [singleton_def, eq_comm]
+
+class Cons (β : outParam Type*) (α : Type*) [Membership β α] where
+  cons : β → α → α
+  mem_cons_iff {x z : β} {a : α} : x ∈ cons z a ↔ x = z ∨ x ∈ a
+
+attribute [simp] Cons.mem_cons_iff
+
+export Cons (cons)
+
+instance (α : Type*) : Cons α (Set α) := ⟨insert, by simp⟩
+
+instance (α : Type*) : Cons α (List α) := ⟨List.cons, by simp⟩
+
+instance (α : Type*) : Cons α (Multiset α) := ⟨Multiset.cons, by simp⟩
+
+instance (α : Type*) [DecidableEq α] : Cons α (Finset α) := ⟨insert, by simp⟩
 
 namespace Collection
 
-variable {β α : Type*} [Collection β α]
+variable {β α : Type*} [Collection β α] [Cons β α]
 
 def set : α → Set β := fun a ↦ {x | x ∈ a}
 
@@ -60,9 +112,9 @@ lemma subset_antisymm {a b : α} (ha : a ⊆ b) (hb : b ⊆ a) : set a = set b :
 
 @[simp] lemma empty_subset (a : α) : ∅ ⊆ a := by simp [subset_iff]
 
-@[simp] lemma mem_cons (a : α) (x : β) : x ∈ cons x a := by simp [mem_cons_iff]
+@[simp] lemma mem_cons (a : α) (x : β) : x ∈ cons x a := by simp
 
-@[simp] lemma subset_cons (a : α) (x : β) : a ⊆ cons x a := by simp [subset_iff, mem_cons_iff]; tauto
+@[simp] lemma subset_cons (a : α) (x : β) : a ⊆ cons x a := by simp [subset_iff]; tauto
 
 @[simp] lemma set_empty : set (∅ : α) = ∅ := by ext; simp [set]
 
